common/LinkingC.v
@@ -155,26 +155,6 @@ Proof.
   - destruct xs; ss.
 Qed.
 
-Lemma link_list_app_commut
-      X `{Linker X}
-      x_link xs0 xs1
-      (LINK: link_list xs1 = Some x_link)
-  :
-    <<CMT: link_list (xs0 ++ xs1) = link_list (xs0 ++ [x_link])>>
-.
-Proof.
-  ginduction xs1; ii; ss.
-  { unfold link_list in LINK. des_ifs. ss. des_ifs.
-    { destruct xs1; ss. des_ifs. }
-    replace (xs0 ++ a :: xs1) with ((xs0 ++ [a]) ++ xs1); cycle 1.
-    { rewrite <- app_assoc. ss. }
-    erewrite IHxs1; et; cycle 1.
-    { unfold link_list. rewrite Heq0. ss. }
-    rewrite <- app_assoc. ss.
-    erewrite link_list_snoc_commut; eauto.
-  }
-Qed.
-
 (* Lemma link_list_cons_commut *)
 (*       X `{Linker X} *)
 (*       x0 x1 x_link xs *)
@@ -183,14 +163,14 @@ Qed.
 (*     <<CMT: link_list (x0 :: x1 :: xs) = link_list (x_link :: xs)>> *)
 (* . *)
 (* Proof. *)
-  
+
 (*   { *)
 (*     remember (rev xs) as rem. *)
 (*     move rem at top. *)
 (*     revert_until H. *)
 (*     ginduction rem; ii; ss. *)
 (*     { hexpl rev_nil. clarify. ss. unfold link_list; ss. des_ifs. } *)
-    
+
 (*   } *)
 (*   ginduction xs; ii; ss. *)
 (*   { unfold link_list. ss. des_ifs. } *)
@@ -200,7 +180,7 @@ Qed.
 (*   { ss. *)
 (*   ss. des_ifs. *)
 (*   exploit IHxs; eauto. i; des. *)
-  
+
 (*   ss. *)
 (* Qed. *)
 
