driver/SepComp.v
@@ -28,15 +28,15 @@ Proof.
 Qed.
 
 Theorem separate_compilation_correct
-        (srcs: list Csyntax.program) (tgts: list Asm.program) src_link
-        (TYPECHECKS: Forall CsemC.typechecked srcs)
-        (TYPECHECKLINK: CsemC.typechecked src_link)
+        (srcs: list Csyntax.program) (tgts: list Asm.program) builtins src_link
+        (TYPECHECKS: Forall (fun src => CsemC.typechecked builtins src) srcs)
+        (TYPECHECKLINK: CsemC.typechecked builtins src_link)
         (LINK: link_list srcs = Some src_link)
         (MAIN: exists main_f,
             (<<INTERNAL: src_link.(prog_defmap) ! (src_link.(prog_main)) = Some (Gfun (Ctypes.Internal main_f))>>)
             /\
             (<<SIG: type_of_function main_f = Tfunction Ctypes.Tnil type_int32s cc_default>>))
-        (TR: Errors.mmap CompilerC.transf_c_program srcs = Errors.OK tgts)
+        (TR: Errors.mmap transf_c_program srcs = Errors.OK tgts)
   :
     (<<INITUB: program_behaves (Csem.semantics src_link) (Goes_wrong E0)>>) \/
     exists tgt_link, <<LINK: link_list tgts = Some tgt_link>> /\
@@ -45,7 +45,9 @@ Theorem separate_compilation_correct
 Proof.
   hexploit upperbound_b_correct; eauto. { des. esplits; et. } intro A.
   hexploit upperbound_a_correct; eauto. instantiate (1:= []). ss. intro B; des.
-  hexploit compiler_correct; eauto. instantiate (1:= []). ss. rewrite ! app_nil_r. intro C; des.
+  hexploit compiler_correct; eauto.
+  { do 2 instantiate (1:= []). ss. }
+  instantiate (1:= []). ss. rewrite ! app_nil_r. intro C; des.
   hexploit (lower_bound_correct tgts); eauto. intro D.
   des.
   { left.
